@prefix : <http://www.semanticweb.org/owl/owlapi/turtle#> .
@prefix owl: <http://www.w3.org/2002/07/owl#> .
@prefix rdf: <http://www.w3.org/1999/02/22-rdf-syntax-ns#> .
@prefix xml: <http://www.w3.org/XML/1998/namespace> .
@prefix skos: <http://www.w3.org/2004/02/skos/core#> .
@prefix vann: <http://purl.org/vocab/vann/> .
@prefix schema: <https://schema.org/> .
@prefix dcterms: <http://purl.org/dc/terms/> .
@prefix xsd: <http://www.w3.org/2001/XMLSchema#> .
@prefix rdfs: <http://www.w3.org/2000/01/rdf-schema#> .
@prefix ssno: <https://matthiasprobst.github.io/ssno> .
@prefix m4i: <http://w3id.org/nfdi4ing/metadata4ing#> .
@prefix pivm: <https://matthiasprobst.github.io/pivmeta#> .
@base <https://matthiasprobst.github.io/pivmeta#> .

<https://matthiasprobst.github.io/pivmeta#> rdf:type owl:Ontology ;
                                               owl:imports <http://w3id.org/nfdi4ing/metadata4ing/1.2.1> ;
                                               dcterms:abstract "This is an ontology draft for the description of Particle Image Velocimetry data. It is currently limited to planar PIV (2D2C and 2D3C) setups."@en ;
                                               dcterms:created "2024-01-03" ;
                                               dcterms:creator "Matthias Probst (https://orcid.org/0000-0001-8729-0482), Institut für Thermische Strömungsmaschinen" ;
                                               dcterms:license <https://creativecommons.org/licenses/by/4.0/> ;
                                               dcterms:modified "2024-01-03" ;
                                               dcterms:title "PIVMeta: An ontology draft for describing particle image velocimetry data."@en ;
                                               vann:preferredNamespacePrefix "pivm" ;
                                               vann:preferredNamespaceUri "https://matthiasprobst.github.io/pivm#" ;
                                               m4i:ContactPerson "https://orcid.org/0000-0001-8729-0482" ;
                                               rdfs:label "PIVMeta" ;
                                               owl:versionInfo "v1.0.0" .

#################################################################
#    Annotation properties
#################################################################

###  http://purl.org/dc/terms/abstract
dcterms:abstract rdf:type owl:AnnotationProperty .


###  http://purl.org/dc/terms/created
dcterms:created rdf:type owl:AnnotationProperty .


###  http://purl.org/dc/terms/creator
dcterms:creator rdf:type owl:AnnotationProperty .


###  http://purl.org/dc/terms/license
dcterms:license rdf:type owl:AnnotationProperty .


###  http://purl.org/dc/terms/modified
dcterms:modified rdf:type owl:AnnotationProperty .


###  http://purl.org/dc/terms/title
dcterms:title rdf:type owl:AnnotationProperty .


###  http://purl.org/vocab/vann/preferredNamespacePrefix
vann:preferredNamespacePrefix rdf:type owl:AnnotationProperty .


###  http://purl.org/vocab/vann/preferredNamespaceUri
vann:preferredNamespaceUri rdf:type owl:AnnotationProperty .


###  http://www.w3.org/2004/02/skos/core#altLabel
<http://www.w3.org/2004/02/skos/core#altLabel> rdf:type owl:AnnotationProperty .


###  http://www.w3.org/2004/02/skos/core#broader
<http://www.w3.org/2004/02/skos/core#broader> rdf:type owl:AnnotationProperty .


###  http://www.w3.org/2004/02/skos/core#closeMatch
<http://www.w3.org/2004/02/skos/core#closeMatch> rdf:type owl:AnnotationProperty .


###  http://www.w3.org/2004/02/skos/core#definition
<http://www.w3.org/2004/02/skos/core#definition> rdf:type owl:AnnotationProperty .


###  http://www.w3.org/2004/02/skos/core#editorialNote
<http://www.w3.org/2004/02/skos/core#editorialNote> rdf:type owl:AnnotationProperty .


###  http://www.w3.org/2004/02/skos/core#example
<http://www.w3.org/2004/02/skos/core#example> rdf:type owl:AnnotationProperty .


###  http://www.w3.org/2004/02/skos/core#note
<http://www.w3.org/2004/02/skos/core#note> rdf:type owl:AnnotationProperty .


###  http://www.w3.org/2004/02/skos/core#prefLabel
<http://www.w3.org/2004/02/skos/core#prefLabel> rdf:type owl:AnnotationProperty .


#################################################################
#    Datatypes
#################################################################

###  http://www.w3.org/2001/XMLSchema#date
xsd:date rdf:type rdfs:Datatype .


###  https://www.w3.org/TR/rdf12-schema/#rdfs:label
<https://www.w3.org/TR/rdf12-schema/#rdfs:label> rdf:type rdfs:Datatype .


#################################################################
#    Object Properties
#################################################################

###  https://matthiasprobst.github.io/ssno#hasStandardName
<https://matthiasprobst.github.io/ssno#hasStandardName> rdf:type owl:ObjectProperty ;
                                                        rdfs:domain <http://w3id.org/nfdi4ing/metadata4ing#NumericalVariable> ;
                                                        rdfs:range <https://matthiasprobst.github.io/ssno#StandardName> ;
                                                        <http://www.w3.org/2004/02/skos/core#prefLabel> "has standard name"@en .


#################################################################
#    Data properties
#################################################################

###  https://matthiasprobst.github.io/pivmeta#final_window_size
:final_window_size rdf:type owl:DatatypeProperty ;
                   rdfs:subPropertyOf owl:topDataProperty ;
                   rdfs:domain pivm:InterrogationMethod ;
                   rdfs:comment "The final window size used by any PIV interrogation method."@en .


###  https://matthiasprobst.github.io/pivmeta#initial_window_size
:initial_window_size rdf:type owl:DatatypeProperty ;
                     rdfs:subPropertyOf owl:topDataProperty ;
                     rdfs:domain pivm:Multigrid ;
                     rdfs:comment "The initial window size used by a Multigrid PIV method."@en .


###  https://matthiasprobst.github.io/pivmeta#number_of_passes
:number_of_passes rdf:type owl:DatatypeProperty ;
                  rdfs:subPropertyOf owl:topDataProperty ;
                  rdfs:domain pivm:Multipass ;
                  rdfs:range xsd:int ;
                  rdfs:comment "The number of passes performed by the Multipass PIV Method."@en .


###  https://matthiasprobst.github.io/pivmeta#percentage_of_final_window_size
:percentage_of_final_window_size rdf:type owl:DatatypeProperty ;
                                 rdfs:subPropertyOf owl:topDataProperty ;
                                 rdfs:domain pivm:InterrogationMethod ;
                                 rdfs:range xsd:float .


#################################################################
#    Classes
#################################################################

###  http://purl.obolibrary.org/obo/BFO_0000017
<http://purl.obolibrary.org/obo/BFO_0000017> rdf:type owl:Class ;
                                             <http://www.w3.org/2004/02/skos/core#definition> "To say that b is a realizable entity is to say that b is a specifically dependent continuant that inheres in some independent continuant which is not a spatial region and is of a type instances of which are realized in processes of a correlated type. (axiom label in BFO2 Reference: [058-002])" ;
                                             <http://www.w3.org/2004/02/skos/core#prefLabel> "realisierbare Entität"@de ,
                                                                                             "realizable entity"@en .


###  http://purl.obolibrary.org/obo/Process
<http://purl.obolibrary.org/obo/Process> rdf:type owl:Class .


###  http://w3id.org/nfdi4ing/metadata4ing#Method
<http://w3id.org/nfdi4ing/metadata4ing#Method> rdf:type owl:Class ;
                                               rdfs:subClassOf <http://purl.obolibrary.org/obo/BFO_0000017> .


###  http://w3id.org/nfdi4ing/metadata4ing#NumericalVariable
<http://w3id.org/nfdi4ing/metadata4ing#NumericalVariable> rdf:type owl:Class .


###  http://w3id.org/nfdi4ing/metadata4ing#ProcessingStep
<http://w3id.org/nfdi4ing/metadata4ing#ProcessingStep> rdf:type owl:Class ;
                                                       rdfs:subClassOf <http://www.w3.org/ns/prov#Activity> .


###  http://w3id.org/nfdi4ing/metadata4ing#Tool
<http://w3id.org/nfdi4ing/metadata4ing#Tool> rdf:type owl:Class .


###  http://www.w3.org/ns/prov#Activity
<http://www.w3.org/ns/prov#Activity> rdf:type owl:Class ;
                                     rdfs:subClassOf <http://purl.obolibrary.org/obo/Process> ;
                                     rdfs:label "Activity"@en .


###  https://matthiasprobst.github.io/pivmeta#CenterOfMass
pivm:CenterOfMass rdf:type owl:Class ;
              rdfs:subClassOf pivm:SubPixelPeakFitMethod .


###  https://matthiasprobst.github.io/pivmeta#InterrogationMethod
pivm:InterrogationMethod rdf:type owl:Class ;
                     rdfs:subClassOf <http://w3id.org/nfdi4ing/metadata4ing#Method> .


###  https://matthiasprobst.github.io/pivmeta#LeastSquaresGauss
pivm:LeastSquaresGauss rdf:type owl:Class ;
                   rdfs:subClassOf pivm:SubPixelPeakFitMethod .


###  https://matthiasprobst.github.io/pivmeta#Multigrid
pivm:Multigrid rdf:type owl:Class ;
           rdfs:subClassOf pivm:InterrogationMethod .


###  https://matthiasprobst.github.io/pivmeta#Multipass
pivm:Multipass rdf:type owl:Class ;
           rdfs:subClassOf pivm:InterrogationMethod .


###  https://matthiasprobst.github.io/pivmeta#PIVProcessingStep
pivm:PIVProcessingStep rdf:type owl:Class ;
                   rdfs:subClassOf <http://w3id.org/nfdi4ing/metadata4ing#ProcessingStep> ;
                   <http://www.w3.org/2004/02/skos/core#definition> "PIV-specific action undertaken during PIV data handling from recording to processing."@en ;
                   <http://www.w3.org/2004/02/skos/core#prefLabel> "piv processing step"@en .


###  https://matthiasprobst.github.io/pivmeta#Singlepass
pivm:Singlepass rdf:type owl:Class ;
            rdfs:subClassOf pivm:InterrogationMethod .


###  https://matthiasprobst.github.io/pivmeta#SubPixelPeakFitMethod
pivm:SubPixelPeakFitMethod rdf:type owl:Class ;
                       rdfs:subClassOf <http://w3id.org/nfdi4ing/metadata4ing#Method> ;
                       rdfs:comment "Method fitting the sub pixel peak in the correlation signal."@en .


###  https://matthiasprobst.github.io/pivmeta#ThreePointParabolic
pivm:ThreePointParabolic rdf:type owl:Class ;
                     rdfs:subClassOf pivm:SubPixelPeakFitMethod .


###  https://matthiasprobst.github.io/pivmeta#ThreePointsGauss
pivm:ThreePointsGauss rdf:type owl:Class ;
                  rdfs:subClassOf pivm:SubPixelPeakFitMethod .


###  https://matthiasprobst.github.io/pivmeta##EvaluationStep
<https://matthiasprobst.github.io/pivmeta##EvaluationStep> rdf:type owl:Class ;
                                                           rdfs:subClassOf pivm:PIVProcessingStep ;
                                                           rdfs:label "evaluation step"@en ;
                                                           <http://www.w3.org/2004/02/skos/core#definition> "The main PIV process which evaluates the pixel displacements."@en .


###  https://matthiasprobst.github.io/pivmeta##PostProcessingStep
<https://matthiasprobst.github.io/pivmeta##PostProcessingStep> rdf:type owl:Class ;
                                                               rdfs:subClassOf pivm:PIVProcessingStep ;
                                                               rdfs:label "post processing step"@en ;
                                                               <http://www.w3.org/2004/02/skos/core#definition> "Processing step which takes place after the main PIV evaluation. It may include outlier detection, interpolation and other manipulating operations."@en .


###  https://matthiasprobst.github.io/pivmeta##PreProcessingStep
<https://matthiasprobst.github.io/pivmeta##PreProcessingStep> rdf:type owl:Class ;
                                                              rdfs:subClassOf pivm:PIVProcessingStep ;
                                                              rdfs:label "pre processing step"@en ;
                                                              <http://www.w3.org/2004/02/skos/core#definition> "Processing step prior to the main processing step including image manipulation, e.g. cropping, rotating or filtering."@en .


###  https://matthiasprobst.github.io/ssno#StandardName
<https://matthiasprobst.github.io/ssno#StandardName> rdf:type owl:Class .


#################################################################
#    Individuals
#################################################################

###  https://matthiasprobst.github.io/pivmeta#estimated_particle_image_density
pivm:estimated_particle_image_density rdf:type owl:NamedIndividual ;
                                  <http://www.w3.org/2004/02/skos/core#definition> "The number of particles per pixel (ppp) estimated by means of an algorithm or by manual counting the particles."@en ;
                                  <http://www.w3.org/2004/02/skos/core#prefLabel> "estimated particle image density"@en .


###  https://matthiasprobst.github.io/pivmeta#measured_particle_density
pivm:measured_particle_density rdf:type owl:NamedIndividual ;
                           <http://www.w3.org/2004/02/skos/core#definition> "The number of particles per volume measured by a measurement device."@en ;
                           <http://www.w3.org/2004/02/skos/core#prefLabel> "measured particle density"@en .


###  https://matthiasprobst.github.io/pivmeta#measured_particle_image_density
pivm:measured_particle_image_density rdf:type owl:NamedIndividual ;
                                 <http://www.w3.org/2004/02/skos/core#definition> "The number of particles per pixel measured by a measurement device."@en ;
                                 <http://www.w3.org/2004/02/skos/core#prefLabel> "measured particle image density"@en .


###  https://matthiasprobst.github.io/pivmeta#quantum_efficiency
pivm:quantum_efficiency rdf:type owl:NamedIndividual ;
                    <http://www.w3.org/2004/02/skos/core#definition> "Quantum efficiency of a digital camera sensor."@en ;
                    <http://www.w3.org/2004/02/skos/core#prefLabel> "quantum efficiency"@en .


###  https://matthiasprobst.github.io/pivmeta#x_displacement
pivm:x_displacement rdf:type owl:NamedIndividual ;
                <http://www.w3.org/2004/02/skos/core#definition> "Approximated displacement of tracer particles determined by a PIV algorithm. Displacement is a vector quantity. X indicates the component in x-axis direction of the respective coordinate system."@en ;
                <http://www.w3.org/2004/02/skos/core#prefLabel> "x displacement"@en .


###  https://matthiasprobst.github.io/pivmeta#x_true_particle_displacement
pivm:x_true_particle_displacement rdf:type owl:NamedIndividual ;
                              rdfs:comment "Note, that tracer particle displacement is generally only known from synthetically generated PIV images."@en ;
                              <http://www.w3.org/2004/02/skos/core#definition> "True displacement of tracer particles. Displacement is a vector quantity. X indicates the component in x-axis direction of the respective coordinate system."@en ;
                              <http://www.w3.org/2004/02/skos/core#prefLabel> "x true particle displacement"@en .


###  https://matthiasprobst.github.io/pivmeta#x_velocity
pivm:x_velocity rdf:type owl:NamedIndividual ;
            <http://www.w3.org/2004/02/skos/core#definition> "Approximated velocity of medium determined by a PIV algorithm based on tracer movement. Velocity is a vector quantity. X indicates the component in x-axis direction of the respective coordinate system."@en ;
            <http://www.w3.org/2004/02/skos/core#prefLabel> "x velocity"@en .


###  https://matthiasprobst.github.io/pivmeta#y_displacement
pivm:y_displacement rdf:type owl:NamedIndividual ;
                <http://www.w3.org/2004/02/skos/core#definition> "Approximated displacement of tracer particles determined by a PIV algorithm. Displacement is a vector quantity. Y indicates the component in y-axis direction of the respective coordinate system."@en ;
                <http://www.w3.org/2004/02/skos/core#prefLabel> "y displacement"@en .


###  https://matthiasprobst.github.io/pivmeta#y_true_particle_displacement
pivm:y_true_particle_displacement rdf:type owl:NamedIndividual ;
                              rdfs:comment "Note, that tracer particle displacement is generally only known from synthetically generated PIV images."@en ;
                              <http://www.w3.org/2004/02/skos/core#definition> "True displacement of tracer particles. Displacement is a vector quantity. Y indicates the component in y-axis direction of the respective coordinate system."@en ;
                              <http://www.w3.org/2004/02/skos/core#prefLabel> "y true particle displacement"@en .


###  https://matthiasprobst.github.io/pivmeta#y_velocity
pivm:y_velocity rdf:type owl:NamedIndividual ;
            <http://www.w3.org/2004/02/skos/core#definition> "Approximated velocity of medium determined by a PIV algorithm based on tracer movement. Velocity is a vector quantity. Y indicates the component in y-axis direction of the respective coordinate system."@en ;
            <http://www.w3.org/2004/02/skos/core#prefLabel> "y velocity"@en .


###  https://matthiasprobst.github.io/pivmeta#z_displacement
pivm:z_displacement rdf:type owl:NamedIndividual ;
                <http://www.w3.org/2004/02/skos/core#definition> "Approximated displacement of tracer particles determined by a PIV algorithm. Displacement is a vector quantity. Z indicates the component in z-axis direction of the respective coordinate system."@en ;
                <http://www.w3.org/2004/02/skos/core#prefLabel> "z displacement"@en .


###  https://matthiasprobst.github.io/pivmeta#z_true_particle_displacement
pivm:z_true_particle_displacement rdf:type owl:NamedIndividual ;
                              rdfs:comment "Note, that tracer particle displacement is generally only known from synthetically generated PIV images."@en ;
                              <http://www.w3.org/2004/02/skos/core#definition> "True displacement of tracer particles. Displacement is a vector quantity. Z indicates the component in z-axis direction of the respective coordinate system."@en ;
                              <http://www.w3.org/2004/02/skos/core#prefLabel> "z true particle displacement"@en .


###  https://matthiasprobst.github.io/pivmeta#z_velocity
pivm:z_velocity rdf:type owl:NamedIndividual ;
            <http://www.w3.org/2004/02/skos/core#definition> "Approximated velocity of medium determined by a PIV algorithm based on tracer movement. Velocity is a vector quantity. Z indicates the component in z-axis direction of the respective coordinate system."@en ;
            <http://www.w3.org/2004/02/skos/core#prefLabel> "z velocity"@en .


###  Generated by the OWL API (version 4.5.26.2023-07-17T20:34:13Z) https://github.com/owlcs/owlapi
